checker/coq/resolution.v
@@ -1,6 +1,6 @@
-(* Resolution of clauses. *)
 Require Import prim.
 Require Lists.List.
+Require Import domain.
 Require Import domset.
 
 (* Actually, we can get away with doing deduplication in a preprocess;
@@ -18,49 +18,257 @@ Fixpoint dedup (cl : clause) :=
   end.
 
 (* FIXME: Implement prop_clause. *)
-Definition prop_clause (ds : domset) (cl : clause) := ds.
-(*
+Definition lit_unsatb (ds : domset) (l : lit) :=
+  match lit_ivar l with
+  | None => false
+  | Some x => dom_unsatb (dom_meet (dom_from_domset ds x) (dom_from_lit x l))
+  end.
+
+Theorem lit_unsatb_valid : forall ds l theta, lit_unsatb ds l = true ->
+  eval_domset ds theta -> ~ eval_lit l theta.
+Proof.
+  intros ds l theta; unfold lit_unsatb.
+  remember (lit_ivar l) as z; destruct z.
+  rewrite dom_unsatb_unsat.
+  intros; intro.
+  set (k := (eval_ivar i theta)).
+  assert (sat_dom (dom_from_domset ds i) k).
+    unfold dom_from_domset.
+    remember (map.ZMaps.find i ds) as f.
+    destruct f; symmetry in Heqf.
+    rewrite eval_domset_alt in H0.
+    apply map.ZMaps.find_2 in Heqf.
+    apply H0 in Heqf.
+    now unfold eval_dom in Heqf.
+
+    apply dom_unconstrained_is_uncon.
+  
+  apply (dom_from_lit_valid i) in H1.
+  assert (sat_dom (dom_meet (dom_from_domset ds i) (dom_from_lit i l)) k).
+  rewrite dom_meet_iff; split; [ assumption | assumption ].
+  now apply H in H3.
+  congruence.
+Qed.
+
+Fixpoint clause_unsatb ds cl :=
   match cl with
-  | nil => ds (* FIXME - should be empty domain. *)
+  | nil => true
+  | cons l cl' => andb (lit_unsatb ds l) (clause_unsatb ds cl')
+  end.
+Theorem clause_unsatb_valid : forall ds cl theta,
+  clause_unsatb ds cl = true -> eval_domset ds theta -> ~ eval_clause cl theta.
+Proof.
+  induction cl.
+    intros; tauto.
+
+  unfold clause_unsatb; fold clause_unsatb;
+  unfold eval_clause; fold eval_clause;
+  intros.
+  intro.
+  rewrite Bool.andb_true_iff in H; destruct H as [Hl Hc].
+  destruct H1.
+    now apply (lit_unsatb_valid ds  a theta) in Hl.
+    now apply IHcl in H.
+Qed.
+
+Definition dom_tighten ds l :=
+  match lit_ivar l with
+  | None => Some ds
+  | Some x =>
+    let d := dom_meet (dom_from_domset ds x) (dom_from_lit x l) in
+    if dom_unsatb d then
+      None
+    else
+      Some (map.ZMaps.add x d ds)
+  end.
+
+Theorem dom_tighten_valid_1 : forall ds ds' l theta,
+  dom_tighten ds l = Some ds' ->
+    eval_domset ds theta -> eval_lit l theta -> eval_domset ds' theta.
+Proof.
+  unfold dom_tighten.
+  intros; destruct (lit_ivar l); try congruence.
+  destruct (dom_unsatb (dom_meet (dom_from_domset ds i) (dom_from_lit i l))); try congruence.
+    inversion H.
+    rewrite eval_domset_alt; intros; simpl.
+
+    apply map.ZMapProperties.F.add_mapsto_iff in H2.
+    destruct H2 as [Hmap | Hmap] ; destruct Hmap as [Hx Hd].
+
+    rewrite <- Hd, Hx; apply eval_dom_meet; split.
+   
+    apply dom_from_domset_valid.
+    apply H0.
+    now apply dom_from_lit_valid.
+    
+    rewrite eval_domset_alt in H0.
+    now apply H0.
+
+    inversion H; now rewrite <- H3.
+Qed.
+
+Theorem dom_tighten_valid_2 : forall ds l theta,
+  dom_tighten ds l = None ->
+    eval_domset ds theta -> ~ eval_lit l theta.
+Proof.
+  unfold dom_tighten.
+  intros ds l theta; destruct (lit_ivar l); try congruence.
+  remember (dom_unsatb (dom_meet (dom_from_domset ds i) (dom_from_lit i l))) as u;
+      destruct u; simpl.
+
+    symmetry in Hequ; rewrite dom_unsatb_unsat in Hequ.
+    intros; intro.
+    assert (sat_dom (dom_meet (dom_from_domset ds i) (dom_from_lit i l)) (eval_ivar i theta)).
+    apply dom_meet_iff; split; [now apply dom_from_domset_valid | now apply dom_from_lit_valid].
+    now apply Hequ in H2. 
+
+    congruence.
+Qed.
+
+Fixpoint prop_clause (ds : domset) (cl : clause) := (* ds. *)
+  match cl with
+  | nil => None
   | cons l cl' =>
-    if lit_unsat ds l then
+    if lit_unsatb ds l then
       prop_clause ds cl'
     else
-      if clause_unsat ds cl' then
-        
+      if clause_unsatb ds cl' then
+        dom_tighten ds l
       else
-        ds
+        Some ds
   end.
-*)
 
-Lemma prop_clause_valid : forall (ds : domset) (cl : clause) (theta : asg),
-    eval_domset ds theta -> eval_domset (prop_clause ds cl) theta.
+Lemma prop_clause_valid_1 : forall (ds ds' : domset) (cl : clause) (theta : asg),
+    (prop_clause ds cl) = Some ds' -> eval_domset ds theta -> eval_clause cl theta -> eval_domset ds' theta.
 Proof.
-  intros; unfold prop_clause; assumption.
+  intros ds ds' cl theta; unfold prop_clause; induction cl; simpl;
+  intros; inversion H.
+  fold prop_clause in *.
+  remember (lit_unsatb ds a) as ul; destruct ul; try congruence.
+  destruct H1 as [Ha | Hcl].
+    symmetry in Hequl; now apply lit_unsatb_valid with (theta := theta) in Hequl.
+
+    apply IHcl in H3; try assumption.
+
+    remember (clause_unsatb ds cl) as uc; destruct uc; try congruence.
+      destruct H1 as [Ha | Hcl].
+
+      apply dom_tighten_valid_1 with (theta := theta) in H3; assumption.
+      symmetry in Hequc; apply clause_unsatb_valid with (theta := theta) in Hequc;
+        [contradiction|assumption].
+      
+      inversion H3; now rewrite <- H4.
+Qed.
+
+Lemma prop_clause_valid_2 : forall (ds : domset) (cl : clause) (theta : asg),
+    (prop_clause ds cl) = None -> eval_domset ds theta -> ~ eval_clause cl theta.
+Proof.
+  unfold prop_clause; intros; induction cl.
+    now unfold eval_clause.
+
+    fold prop_clause in *.
+    unfold eval_clause; fold eval_clause; intro.
+
+    remember (lit_unsatb ds a) as ua; remember (clause_unsatb ds cl) as uc.
+    destruct ua; symmetry in Hequa.
+    destruct H1.
+      now apply lit_unsatb_valid with (theta := theta) in Hequa.
+
+      now apply IHcl in H.
+
+    destruct uc; symmetry in Hequc.
+      destruct H1 as [Ha | Hcl];
+      [now apply dom_tighten_valid_2 with (theta := theta) in H |
+       now apply clause_unsatb_valid with (theta := theta) in Hequc].
+    congruence.
 Qed.
 
 Fixpoint unit_prop (ds : domset) (cs : list clause) :=
   match cs with
-  | nil => ds
+  | nil => Some ds
   | cons cl cs' =>
-      prop_clause (unit_prop (prop_clause ds cl) cs') cl
+    match prop_clause ds cl with
+    | None => None
+    | Some ds' =>
+      match unit_prop ds' cs' with
+      | None => None
+      | Some ds'' =>
+        prop_clause ds'' cl
+      end
+    end
   end.
-Lemma unit_prop_valid : forall (ds : domset) (cs : list clause) (theta : asg),
-  eval_domset ds theta -> eval_domset (unit_prop ds cs) theta.
-Proof.
-  unfold unit_prop; intros; induction cs.
-    assumption.
-    fold unit_prop in *.
-    apply prop_clause_valid; apply IHcs; now apply prop_clause_valid.
-Qed.
-  
 
-(* FIXME: Implement resolvable. *)
-Definition resolvable (cl : clause) (ants : list clause) :=
-  false.
+Lemma unit_prop_valid_1 : forall (cs : list clause) (theta : asg),
+  (* unit_prop ds cs = Some ds' -> eval_domset ds theta -> eval_clauses cs theta ->
+    eval_domset ds' theta. *)
+  eval_clauses cs theta -> forall ds, eval_domset ds theta ->
+    forall ds', unit_prop ds cs = Some ds' -> eval_domset ds' theta.
+Proof.
+  induction cs;
+  unfold unit_prop; intros; simpl in *; fold unit_prop in *.
+    inversion H1; now rewrite <- H3.
+
+  remember (prop_clause ds a) as pds; destruct pds; try congruence.
+  remember (unit_prop t cs) as u; destruct u; try congruence.
+  destruct H as [Ha Hcs].
+  apply prop_clause_valid_1 with (ds := d) (cl := a); try assumption.
+  symmetry in Hequ, Heqpds.
+  apply IHcs with (ds := t); try assumption.
+  apply prop_clause_valid_1 with (ds := ds) (cl := a); assumption.
+Qed.
+
+Lemma unit_prop_valid_2 : forall (cs : list clause) (theta : asg),
+  eval_clauses cs theta -> forall ds, unit_prop ds cs = None -> eval_domset ds theta -> False.
+Proof.
+  induction cs; unfold eval_clauses; simpl; intros; fold eval_clauses in *.
+    discriminate.
+
+    destruct H as [Ha Hcs].
+    remember (prop_clause ds a) as pa; destruct pa; try congruence; symmetry in Heqpa.
+    remember (unit_prop t cs) as ut; destruct ut; try congruence; symmetry in Hequt.
+    assert (eval_domset d theta).
+      apply unit_prop_valid_1 with (ds := t) (ds' := d) (cs := cs); try assumption.
+      apply prop_clause_valid_1 with (ds := ds) (cl := a); try assumption.
+    assert (Hp := prop_clause_valid_2 d a theta).
+    tauto.
+
+    apply IHcs with (theta := theta) (ds := t); try assumption.
+    apply prop_clause_valid_1 with (ds := ds) (cl := a); try assumption.
+    assert (~ eval_clause a theta).
+      apply prop_clause_valid_2 with (ds := ds) (cl := a); try assumption.
+      tauto.
+Qed.
+
+(*
+Definition resolvable (cl : clause) (ants : list clause) := false.
 
 Theorem resolvable_valid : forall cl ants,
   resolvable cl ants = true -> forall theta, eval_clauses ants theta -> eval_clause cl theta.
 Proof.
-  intros cl ants; unfold resolvable; discriminate.
+  unfold resolvable; intros; congruence.
 Qed.
+*)
+Definition resolvable (cl : clause) (ants : list clause) :=
+  let ds := negcl_domset cl in
+  match unit_prop ds ants with
+  | None => true
+  | Some _ => false
+  end.
+
+Theorem resolvable_valid : forall cl ants,
+  resolvable cl ants = true -> forall theta, eval_clauses ants theta -> eval_clause cl theta.
+Proof.
+  unfold resolvable; intros.
+  remember (unit_prop (negcl_domset cl) ants) as u; symmetry in Hequ; destruct u;
+    simpl in *; try congruence.
+  clear H.
+  remember (negcl_domset cl) as ds.
+  assert (eval_domset ds theta -> False).
+  apply unit_prop_valid_2 with (cs := ants); try assumption.
+  apply evalclause_contra; intros.
+  apply H.
+  rewrite Heqds.
+  now apply eval_negcl_domset.
+Qed.
+
+(* *)
